# Week 6 - Integration {#ch:Workshop6}

## Preliminary infomation {#sec:Prelim6}

When introducing rearranging of equations in Chapters \@ref(ch:Workshop1) and \@ref(ch:Workshop2) we introduce the idea of inverse functions, and every function has an inverse. With differentiation the inverse process is integration, and as such if we differentiate a function, and then integrate the answer, we should end up with our original function again. Or if we integrate a function, then differentiate the answer we should again end up with our original function.

Our integral can also be thought of as a mechanism of determining the area under a line in a plot, (or between the function and the $x$-axis). There are a number of cases whereby determining the area under a line can give us more infomation about the system. For example the area under a '$pV$' plot is work done in changing the volume ((Section)Figure \@ref(fig:integral), see CH10137 thermodynamics).

```{r echo=FALSE, integral, out.width='50%', fig.show='hold', fig.align='center', fig.cap='Integration can be used to determine the area under a line in a plot. In the case of a pressure-volume plot the area under the plot is the work done in the expansion between the initial and final volume.'}
knitr::include_graphics("images/integral.png")
```

If we aren't considering the area under the line between -∞ & ∞ we need to define the points on the $x$ axis of interest, these are often referred to as 'initial' and 'final'. In this case we call it a 'definite integral'. We can see an example of these in Section \@ref(subsec:definite).


Just like with integration we have a set of standard results, these are the integrals or anti-derivatives:

### Integrating polynomials {#subsec:integratingpolynomials}

If we recall Section \@ref(subsec:diffpolynomial), we saw that when we differentiated a polynomial we reduced the power by one and multiplied by the old power.

\begin{equation*}
y = ax^b\\
\frac{\textrm{d}y}{\textrm{d}x}=abx^{b-1}\\
\textrm{when } x \neq 0
\end{equation*}

To 'undo' this result we need to add one to the power and divide by the new power.

\begin{equation*}
\frac{\textrm{d}y}{\textrm{d}x}=abx^{b-1}\\
y = ax^b\\
\textrm{when } x \neq -1
\end{equation*}

However, if we had a slightly different function that we have differentiated, where $c$ is a constant:

\begin{equation*}
y = ax^b+ c\\
\frac{\textrm{d}y}{\textrm{d}x}=abx^{b-1}\\
\textrm{when } x \neq 0
\end{equation*}

but when we 'undo' this we have nothing to tell us that there used to be a constant there and so whenever we determine integrals (or anti-derivatives) we have to add a constant of integration, $+C$. So, to get back to our 'original function':

\begin{equation*}
\frac{\textrm{d}y}{\textrm{d}x}=abx^{b-1}\\
y = ax^b+C\\
\textrm{when } x \neq -1
\end{equation*}



Instead of just thinking about this as undoing the differential we can instead use our 'integral notation'. Integrals are represented by the sign $\int$, but we also need to know what we are integrating with respect to, and so at the end of our integration statement we use '$\textrm{d}x$' to define what we are integrating with respect to, in this case $x$.

:::dodo
\begin{equation}
\int ax^b \textrm{d}x = \frac{a}{b+1}x^{b+1}+C
(\#eq:intpoly)
\end{equation}

:::

### Integrating exponentials {#subsec:integratingexponentials}

Again if we think about integration as an anti-derivative, we can start by looking back on the result when we differentiated exponential functions in Section \@ref(subsec:diffexp).

\begin{equation*}
y = be^{ax}\\
\frac{\textrm{d}y}{\textrm{d}x}=abe^{ax}
\end{equation*}

and so, integrating:

\begin{equation*}
\frac{\textrm{d}y}{\textrm{d}x}=abe^{ax}\\
y = be^{ax}+C
\end{equation*}

This again makes sense if we look at the Maclaurin expansion of an exponential function Section \@ref(sec:maclaurin).

:::dodo
\begin{equation}
\int ae^{bx} \textrm{d}x = \frac{a}{b}e^{bx}+C
(\#eq:intpoly)
\end{equation}

:::

:::info
\begin{equation*}
\begin{array}{cccc}
f^{\prime}(x) \equiv y & & f(x) \equiv \int y ~\textrm{d}x & \textrm{Conditions}\\
  \hline
  \hline
A & & x + C \\ 
Ax^n & & \dfrac{A}{n+1}x^{n+1}+ C & x \neq -1\\ 
\dfrac{A}{x} \equiv A x^{-1} & &  A \ln x + C\\  
\dfrac{A}{Bx+ d} & & \dfrac{A}{B} \ln(Bx + d) +C\\ 
e^{Ax} & &\frac{1}{A} e^{Ax} + C\\
A^x && \frac{A^x}{\ln A} +C\\
A \ln x & & A \left( x \ln x - x \right)+ C\\

\sin Ax & &-\frac{1}{A}\cos Ax + C\\ 
\cos Ax & &\frac{1}{A}\sin Ax + C\\
\tan Ax & &-\frac{1}{A}\ln(\cos Ax) + C \equiv \frac{1}{A}\ln(\sec Ax) + C & -\frac{\pi}{2} < x < \frac{\pi}{2}\\

\frac{A}{x^2 + B^2} && \frac{A}{B}\tan^{-1}\left(\frac{x}{B}\right) + C &B>0\\
Ax^2 e^{Bx} && A\left(\frac{x^2}{B} - \frac{2x}{B^2} + \frac{2}{B^3} \right)e^{Bx} +C\\

v(x) \frac{\textrm{d}u(x)}{\textrm{d}x} && u(x)v(x) - \int u(x)\frac{\textrm{d}v(x)}{\textrm{d}x} +C & \textrm{Integration by Parts}\\

Au + Bv & &A\dfrac{\textrm{d}u}{\textrm{d}x} + B\dfrac{\textrm{d}v}{\textrm{d}x} \\
\end{array}
\end{equation*}
:::

## Questions {#sec:Questions6}

### Basic integration practice

Integrate the following with respect to the variable specified:

1. $f'(x) = \frac{a}{x}$; x
1. $f'(x) = x^\frac{3}{2}+ \frac{x^\frac{1}{2}}{2} - 2x^{-\frac{1}{2}}$, x
1. $f'(b) = \sin (ab)$; b
1. $f'(T) = a + bT + \frac{c}{T}$; T
1. $f'(t) = k$; t
1. $f'([A]) = \frac{1}{[A]}$, [A]
1. $f'([A]) = \frac{1}{[A]^2}$, [A]
1. $f'(t) = -e^{-kt}$, t

### Differential equations

Solve the following differential equations as far as possible:

1. $\frac{\textrm{d}\ln a}{\textrm{d}z}= bz^2$
1. $\frac{\textrm{d}[A]}{\textrm{d}t} = -k[A]^2$, when t= 0, [A] = [A]~0~
1. $\frac{\textrm{d}p}{\textrm{d}T}=\frac{p\Delta_{\textrm{vap}}H}{RT^2}$; when T = T~1~, p = p~1~ and when when T = T~2~, p = p~2~
1. $\frac{\textrm{d}w}{\textrm{d}V}= -\frac{nRT}{V}$, when V = V~i~, w = 0 and when V = V~f~, w = w

## Answers {#sec:Answers6}

### Basic integration practice

1. $f (x) = a \ln x + C$
1. $f(x) = \frac{2}{5} x^{\frac{5}{2}}+ \frac{x^{\frac{3}{2}}}{3}+4x^{\frac{1}{2}}+C$
1. $f(b) =-\frac{1}{a}\cos (ab) + C$
1. $f(T) = aT + \frac{bT^2}{2} + c\ln T + C$
1. $f(t) = kt +C$
1. $f([A])= \ln [A] + C$
1. $f([A])=-\frac{1}{[A]}+ C$ 
1. $f(t) = \frac{e^{-kt}}{k}$

### Differential equations

1. $\ln a = \frac{bz^3}{3}+D$
1. $\frac{1}{[A]}=\frac{1}{[A]_0}+ kt$
1. $\ln \frac{p_1}{p_2}=\frac{\Delta_{\textrm{vap}}H}{R}\left({\frac{1}{T_2}-\frac{1}{T_1}}\right)$
1. $w = -nRT \ln \frac{V_f}{V_i}$
